Store whole crash-recovery execution in spec invariant.
Proof rules for using the spec assertions are the same, but the invariant just
stores the whole execution history, including from previous crashes. As long as
crashes are observable via trace events, this is good enough and should make
the refinement theorem easier to state and prove.

src/program_logic/spec_assert.v
@@ -3,6 +3,7 @@ From iris.base_logic.lib Require Import invariants.
 From iris.proofmode Require Import tactics.
 From iris.program_logic Require Export language.
 From iris.program_logic Require Import lifting.
+From Perennial.program_logic Require Export crash_lang.
 
 (*
 
@@ -15,6 +16,7 @@ From iris.program_logic Require Import lifting.
 
 Section ghost.
 Context {Λ: language}.
+Context {CS: crash_semantics Λ}.
 
 (** The CMRA for the heap of the specification. *)
 Definition tpoolUR : ucmraT := gmapUR nat (exclR (exprO Λ)).
@@ -53,25 +55,31 @@ Section ghost_spec.
   Definition source_pool_map (tp: gmap nat (language.expr Λ)) : iProp Σ :=
     own cfg_name (◯ (Excl <$> tp : tpoolUR, ε)).
 
+  (*
   Definition safe (ρ: cfg Λ) :=
     ∀ t2 σ2 e2, rtc erased_step ρ (t2, σ2) → e2 ∈ t2 → not_stuck e2 σ2.
+   *)
 
-  Definition source_inv tp σ : iProp Σ :=
-    (∃ tp' σ', own cfg_name (● (tpool_to_res tp', Some (Excl σ'))) ∗
-                   ⌜ rtc erased_step (tp, σ) (tp', σ')
-                     ∧ safe (tp, σ) ⌝)%I.
+  Definition crash_safe r (ρ: cfg Λ) :=
+    ∀ t2 σ2 e2 s, erased_rsteps (CS := CS) r ρ (t2, σ2) s →
+                  e2 ∈ t2 → not_stuck e2 σ2.
 
-  Definition source_ctx' ρ : iProp Σ :=
-    inv sourceN (source_inv (fst ρ) (snd ρ)).
+  Definition source_inv r tp σ : iProp Σ :=
+    (∃ s tp' σ', own cfg_name (● (tpool_to_res tp', Some (Excl σ'))) ∗
+                   ⌜ erased_rsteps (CS := CS) r (tp, σ) (tp', σ') s
+                     ∧ crash_safe r (tp, σ) ⌝)%I.
+
+  Definition source_ctx' r ρ : iProp Σ :=
+    inv sourceN (source_inv r (fst ρ) (snd ρ)).
 
   Definition source_ctx : iProp Σ :=
-    (∃ ρ, source_ctx' ρ)%I.
+    (∃ r ρ, source_ctx' r ρ)%I.
 
   Global Instance tpool_mapsto_timeless j e : Timeless (tpool_mapsto j e).
   Proof. apply _. Qed.
   Global Instance source_state_timeless σ : Timeless (source_state σ).
   Proof. apply _. Qed.
-  Global Instance source_ctx'_persistent ρ : Persistent (source_ctx' ρ).
+  Global Instance source_ctx'_persistent r ρ : Persistent (source_ctx' r ρ).
   Proof. apply _. Qed.
   Global Instance source_ctx_persistent : Persistent (source_ctx).
   Proof. apply _. Qed.
@@ -224,9 +232,9 @@ Section ghost_step.
     * by left.
   Qed.
 
-  Lemma source_cfg_init `{cfgPreG Σ} tp σ :
-    safe (tp, σ) →
-    (|={⊤}=> ∃ _ : cfgG Σ, source_ctx' (tp, σ)
+  Lemma source_cfg_init `{cfgPreG Σ} r tp σ :
+    crash_safe r (tp, σ) →
+    (|={⊤}=> ∃ _ : cfgG Σ, source_ctx' r (tp, σ)
                                        ∗ source_pool_map (tpool_to_map tp) ∗ source_state σ)%I.
   Proof.
     intros Hno_err.
@@ -242,9 +250,9 @@ Section ghost_step.
     }
     set (IN := {| cfg_name := γ |}).
     iExists IN.
-    iMod (inv_alloc sourceN ⊤ (source_inv tp σ) with "[Hauth]").
-    { rewrite /source_inv. iNext. iExists tp, σ. iFrame "Hauth".
-      iPureIntro; split; eauto. econstructor. }
+    iMod (inv_alloc sourceN ⊤ (source_inv r tp σ) with "[Hauth]").
+    { rewrite /source_inv. iNext. iExists Normal,tp, σ. iFrame "Hauth".
+      iPureIntro; split; eauto. econstructor. econstructor. }
     iModIntro. iFrame.
     rewrite pair_split.
     iDestruct "Hfrag" as "($&$)".
@@ -339,14 +347,14 @@ Section ghost_step.
     apply Excl_included in Hstate; setoid_subst; auto.
   Qed.
 
-  Lemma ghost_step_lifting' E ρ j K `{LanguageCtx Λ K} e1 σ1 κ σ2 e2 efs:
+  Lemma ghost_step_lifting' E r ρ j K `{LanguageCtx Λ K} e1 σ1 κ σ2 e2 efs:
     language.prim_step e1 σ1 κ e2 σ2 efs →
     nclose sourceN ⊆ E →
-    source_ctx' ρ ∗ j ⤇ K e1 ∗ source_state σ1
+    source_ctx' r ρ ∗ j ⤇ K e1 ∗ source_state σ1
       ={E}=∗ j ⤇ K e2 ∗ source_state σ2 ∗ [∗ list] ef ∈ efs, ∃ j', j' ⤇ ef.
   Proof.
     iIntros (Hstep ?) "(#Hctx&Hj&Hstate)". rewrite /source_ctx/source_inv.
-    iInv "Hctx" as (tp' σ') ">[Hauth %]" "Hclose".
+    iInv "Hctx" as (s' tp' σ') ">[Hauth %]" "Hclose".
 
     (* Reconcile view based on authoritative element *)
     iDestruct (source_thread_reconcile with "Hj Hauth") as %Heq_thread.
@@ -360,9 +368,9 @@ Section ghost_step.
 
     (* Restore the invariant *)
     iMod ("Hclose" with "[Hauth]").
-    { iNext. iExists (<[j := K e2]>tp' ++ efs), σ2.
+    { iNext. iExists s', (<[j := K e2]>tp' ++ efs), σ2.
       iFrame. intuition. iPureIntro; split; auto.
-      eapply rtc_r; eauto.
+      eapply erased_rsteps_r_1; eauto.
       eapply fill_step in Hstep.
       econstructor. econstructor; eauto.
       - f_equal. symmetry. eapply take_drop_middle; eauto.
@@ -384,7 +392,7 @@ Section ghost_step.
       ={E}=∗ j ⤇ K e2 ∗ source_state σ2 ∗ [∗ list] ef ∈ efs, ∃ j', j' ⤇ ef.
   Proof.
     iIntros (??) "Hj Hsrc ?".
-    iDestruct "Hsrc" as (?) "Hsrc".
+    iDestruct "Hsrc" as (??) "Hsrc".
     iApply ghost_step_lifting'; eauto. iFrame.
   Qed.
 
@@ -401,13 +409,13 @@ Section ghost_step.
     }
     clear Hstuck.
     rewrite /source_ctx/source_inv.
-    iDestruct "Hctx" as (ρ) "#Hctx".
-    iInv "Hctx" as (tp' σ') ">[Hauth Hpure]" "Hclose".
+    iDestruct "Hctx" as (? ρ) "#Hctx".
+    iInv "Hctx" as (? tp' σ') ">[Hauth Hpure]" "Hclose".
     iDestruct "Hpure" as %(Hstep&Hnoerr).
     iDestruct (source_thread_reconcile with "Hj Hauth") as %Heq_thread.
     iDestruct (source_state_reconcile with "Hstate Hauth") as %Heq_state.
     subst.
-    exfalso. rewrite /safe in Hnoerr.
+    exfalso. rewrite /crash_safe in Hnoerr.
     eapply not_not_stuck in Hstuck'.
     eapply Hstuck', Hnoerr; eauto.
     by eapply elem_of_list_lookup_2.
@@ -419,8 +427,8 @@ Section ghost_step.
     source_ctx ∗ j ⤇ K e1
       ={E}=∗ j ⤇ K e2 ∗ [∗ list] ef ∈ efs, ∃ j', j' ⤇ ef.
   Proof.
-    iIntros (Hstep ?) "(#Hctx&Hj)". iDestruct "Hctx" as (?) "Hctx". rewrite /source_ctx/source_inv.
-    iInv "Hctx" as (tp' σ') ">[Hauth %]" "Hclose".
+    iIntros (Hstep ?) "(#Hctx&Hj)". iDestruct "Hctx" as (??) "Hctx". rewrite /source_ctx/source_inv.
+    iInv "Hctx" as (? tp' σ') ">[Hauth %]" "Hclose".
 
     (* Reconcile view based on authoritative element *)
     iDestruct (source_thread_reconcile with "Hj Hauth") as %Heq_thread.
@@ -432,9 +440,9 @@ Section ghost_step.
 
 
     iMod ("Hclose" with "[Hauth]").
-    { iNext. iExists (<[j := K e2]>tp' ++ efs), _.
+    { iNext. iExists _, (<[j := K e2]>tp' ++ efs), _.
       iFrame. intuition. iPureIntro; split; auto.
-      eapply rtc_r; eauto.
+      eapply erased_rsteps_r_1; eauto.
       edestruct Hstep as (?&Hstep').
       eapply fill_step in Hstep'.
       econstructor. econstructor; eauto.
@@ -505,3 +513,4 @@ End ghost_step.
 End ghost.
 
 Notation "j ⤇ e" := (tpool_mapsto j e) (at level 20) : bi_scope.
+
